sec/Semantics.thy
@@ -2,103 +2,224 @@ theory Semantics
   imports "../Soundness"
 begin
 
-datatype pair_sem_st = Terminated | Running | CrashLeak | CrashPair
+datatype run_st = Running | Terminated | Crashed
 
-type_synonym 's ptrace = \<open>'s list \<times> pair_sem_st\<close>
+type_synonym 's ptrace = \<open>'s list \<times> run_st\<close>
+
+
+type_synonym ('a,'b) rgstate = \<open>(('a \<times> 'a) \<times> ('b \<times> 'b))\<close>
+
+type_synonym ('a,'b) secstate = \<open>(('a \<times> 'b) \<times> ('a \<times> 'b))\<close>
+
+datatype 'a rgact = Loc 'a | Env
+
+abbreviation \<open>LocVis a \<equiv> Loc (Vis a)\<close>
+abbreviation \<open>LocTau \<equiv> Loc Tau\<close>
+
+
+datatype ('s, 'a) alist1 = AInit 's | ACons 's 'a \<open>('s, 'a) alist1\<close>
+
+fun ahd :: \<open>('s, 'a) alist1 \<Rightarrow> 's\<close> where
+  \<open>ahd (AInit s) = s\<close>
+| \<open>ahd (ACons s _ _) = s\<close>
+
+fun ahd_act :: \<open>('s, 'a) alist1 \<Rightarrow> 'a\<close> where
+  \<open>ahd_act (AInit _) = undefined\<close>
+| \<open>ahd_act (ACons _ a _) = a\<close>
+
+
+section \<open> relational lifting \<close>
+
+definition
+  \<open>exch4 \<equiv> \<lambda>((a,b),(c,d)). ((a,c),(b,d))\<close>
+
+lemma exch4_apply[simp]:
+  \<open>exch4 ((a,b),(c,d)) = ((a,c),(b,d))\<close>
+  by (simp add: exch4_def)
+
+
+definition twoPredLift :: \<open>('a \<Rightarrow> bool) \<Rightarrow> ('b \<Rightarrow> bool) \<Rightarrow> ('a \<times> 'b \<Rightarrow> bool)\<close> where
+  \<open>twoPredLift p q \<equiv> \<lambda>(x,y). p x \<and> q y\<close>
+
+nonterminal twoPredLiftL
+
+syntax
+  "_twoPredLiftS"  :: "('a \<Rightarrow> bool) \<Rightarrow> twoPredLiftL"  ("\<lblot> _" [0] 1000)
+  "_twoPredLiftC"  :: "twoPredLiftL \<Rightarrow> ('a \<Rightarrow> 'a \<Rightarrow> bool)"  ("_ \<rblot>" [0] 1000)
+  "_twoPredLiftL"  :: "twoPredLiftL \<Rightarrow> ('a \<Rightarrow> 'b \<Rightarrow> bool)"  ("_ \<bar>" [0] 1000)
+  "_twoPredLiftLR"  :: "twoPredLiftL \<Rightarrow> ('b \<Rightarrow> bool) \<Rightarrow> ('a \<Rightarrow> 'b \<Rightarrow> bool)"  ("_ \<bar> _ \<rblot>" [0] 1000)
+  "_twoPredLiftR"  :: "('b \<Rightarrow> bool) \<Rightarrow> ('a \<Rightarrow> 'b \<Rightarrow> bool)"  ("\<bar> _ \<rblot>" [0] 1000)
+
+translations
+  "_twoPredLiftC (_twoPredLiftS p)" \<rightharpoonup> "(CONST twoPredLift) p p"
+  "_twoPredLiftLR (_twoPredLiftS p) q" \<rightleftharpoons> "(CONST twoPredLift) p q"
+  "_twoPredLiftL (_twoPredLiftS p)" \<rightharpoonup> "(CONST twoPredLift) p \<top>"
+  "_twoPredLiftR q" \<rightharpoonup> "(CONST twoPredLift) \<top> q"
+
+
+definition sec_agree
+  :: \<open>('a \<Rightarrow> 'v) \<Rightarrow> 'a \<times> 'a \<Rightarrow> bool\<close> (\<open>\<bbbA>\<close>)
+  where
+    \<open>\<bbbA> vf \<equiv> (\<lambda>(ab,ab'). vf ab = vf ab')\<close>
+
+lemma conj_agree_iff:
+  \<open>\<bbbA> v1 \<sqinter> \<bbbA> v2 = \<bbbA> (\<lambda>x. (v1 x, v2 x))\<close>
+  by (simp add: sec_agree_def exch4_def comp_def fun_eq_iff split: prod.splits)
+
+lemma eqrel_times_eqrel_eq[simp]:
+  \<open>((=) \<times>\<^sub>R (=)) = (=)\<close>
+  by (force simp add: rel_Times_def)
+
+abbreviation(input) \<open>liftP p \<equiv> \<lblot> p \<rblot>\<close>
+definition \<open>liftR r \<equiv> \<lambda>(x,x') (y,y'). r x y \<and> r x' y'\<close>
+
+fun liftC :: \<open>('l \<times> 's \<Rightarrow> 'v) \<Rightarrow> ('l \<times> 's, 'a) comm \<Rightarrow> (('l, 's) rgstate, unit) comm\<close> where
+  \<open>liftC f Skip = Skip\<close>
+| \<open>liftC f (c1 ;; c2) = liftC f c1 ;; liftC f c2\<close>
+| \<open>liftC f (c1 \<parallel> c2) = liftC f c1 \<parallel> liftC f c2\<close>
+| \<open>liftC f (c1 \<^bold>+ c2) = liftC f c1 \<^bold>+ liftC f c2\<close>
+| \<open>liftC f (c1 \<box> c2) = liftC f c1 \<box> liftC f c2\<close>
+| \<open>liftC f \<langle>p, q\<rangle> = \<langle>(liftP p \<sqinter> \<bbbA> f) \<circ> exch4, liftR q \<circ>\<^sub>2 exch4\<rangle>\<close>
+| \<open>liftC f (DO c OD) = DO liftC f c OD\<close>
+
+definition fr_opstep
+  :: \<open>('l::pre_perm_alg \<times> 's \<Rightarrow> bool) \<Rightarrow>
+      unit act \<Rightarrow>
+      ('l \<times> 's, unit) pstate \<Rightarrow>
+      ('l \<times> 's, unit) cpstate \<Rightarrow>
+      bool\<close>
+  where
+  \<open>fr_opstep F \<alpha> sc sc' \<equiv>
+    \<comment> \<open> plain opstep \<close>
+    sc \<midarrow>\<alpha>\<rightarrow> sc' \<or>
+    \<comment> \<open> framed opstep \<close>
+    (case sc of ((hl, hs), c) \<Rightarrow>
+      \<exists>hlf.
+        F (hlf, hs) \<and>
+        hl ## hlf \<and>
+        (case sc' of
+          (Inl (hl', hs'), c') \<Rightarrow>
+            hl' ## hlf \<and>
+            (\<alpha> = Tau \<longrightarrow> hl' = hl) \<and>
+            ((hl + hlf, hs), c) \<midarrow>\<alpha>\<rightarrow> (Inl (hl' + hlf, hs'), c')
+        | (Inr (), c') \<Rightarrow> 
+            ((hl + hlf, hs), c) \<midarrow>\<alpha>\<rightarrow> (Inr (), c'))
+    )\<close>
+
+abbreviation pretty_fr_opstep :: \<open>_ \<Rightarrow> _ \<Rightarrow> _ \<Rightarrow> _ \<Rightarrow> _\<close> (\<open>_ \<midarrow>(_, _)\<rightarrow> _\<close> [60,0,0,60] 60) where
+  \<open>s \<midarrow>F, \<beta>\<rightarrow> s' \<equiv> fr_opstep F \<beta> s s'\<close>
+
+abbreviation pretty_no_fr_opstep :: \<open>_ \<Rightarrow> _ \<Rightarrow> bool\<close> (\<open>_ \<midarrow>(_, |)\<rightarrow>\<close> [60,0] 60) where
+  \<open>s \<midarrow>F, |\<rightarrow> \<equiv> \<forall>\<beta> s'. \<not> fr_opstep F \<beta> s s'\<close>
 
 
 text \<open>
   Note the the most recent state is at the *head* of the list.
-  e.g. [sn, s{n-1}, ..., s1, s0]
+  e.g. [sn, s{n-1}, ..., s1, s0].
+
+  This is a partial trace semantics, in the style of Aczel, where environment moves are represented
+  in the trace.
 \<close>
-inductive pair_trsem
-  :: \<open>('l \<times> 's \<Rightarrow> bool) \<Rightarrow>
+inductive trsem'
+  :: \<open>('l::pre_perm_alg \<times> 's \<Rightarrow> bool) \<Rightarrow>
+      ('l \<times> 's \<Rightarrow> bool) \<Rightarrow>
       ('s \<Rightarrow> 's \<Rightarrow> bool) \<Rightarrow>
-      ('l::pre_perm_alg \<times> 's \<Rightarrow> bool) \<Rightarrow>
-      (('l \<times> 's, unit) pstate \<times> ('l \<times> 's, unit) pstate) ptrace \<Rightarrow>
+      ('s \<Rightarrow> 's \<Rightarrow> bool) \<Rightarrow>
+      ('l \<times> 's \<Rightarrow> bool) \<Rightarrow>
+      ('l \<times> 's \<Rightarrow> bool) \<Rightarrow>
+      ('l \<times> 's, unit) comm \<Rightarrow>
+      ('l \<times> 's, unit) comm \<Rightarrow>
+      (('l \<times> 's) \<times> run_st, unit act rgact) alist1 \<Rightarrow>
       bool\<close>
   where
-    init: \<open>pair_trsem q r F ([xy], Running)\<close>
-  | rely_step_left:
-    \<open>pair_trsem q r F (t, Running) \<Longrightarrow>
-      hd t = (((l1,s1),c1), sc2) \<Longrightarrow>
-      r s1 s1' \<Longrightarrow>
-      pair_trsem q r F ((((l1,s1'),c1), sc2) # t, Running)\<close>
-  | rely_step_right:
-    \<open>pair_trsem q r F (t, Running) \<Longrightarrow>
-      hd t = (sc1, ((l2,s2),c2)) \<Longrightarrow>
-      r s2 s2' \<Longrightarrow>
-      pair_trsem q r F ((sc1, ((l2,s2'),c2)) # t, Running)\<close>
-  | left_plain_step:
-    \<open>pair_trsem q r F (t, Running) \<Longrightarrow>
-      hd t = (sc1, sc2) \<Longrightarrow>
-      sc1 \<midarrow>a\<rightarrow> (Inl s1', c1') \<Longrightarrow>
-      pair_trsem q r F (((s1', c1'), sc2) # t, Running)\<close>
-  | right_plain_step:
-    \<open>pair_trsem q r F (t, Running) \<Longrightarrow>
-      hd t = (sc1, sc2) \<Longrightarrow>
-      sc2 \<midarrow>a\<rightarrow> (Inl s2', c2') \<Longrightarrow>
-      pair_trsem q r F ((sc1, (s2', c2')) # t, Running)\<close>
-  | left_framed_step:
-    \<open>pair_trsem q r F (t, Running) \<Longrightarrow>
-      hd t = (((hl1,hs1),c1), sc2) \<Longrightarrow>
-      F (hlf1, hs1) \<Longrightarrow>
-      hl1 ## hlf1 \<Longrightarrow>
-      ((hl1 + hlf1, hs1), c1) \<midarrow>\<alpha>\<rightarrow> (Inl (hlhlf1', hs1'), c1') \<Longrightarrow>
-      (\<exists>hl1'.
-          hl1' ## hlf1 \<and>
-          hlhlf1' = hl1' + hlf1 \<and>
-          (\<alpha> = Tau \<longrightarrow> hl1' = hl1) \<and>
-          t' = (((hl1',hs1'),c1'), sc2) # t) \<Longrightarrow>
-      pair_trsem q r F (t', Running)\<close>
-  | right_framed_step:
-    \<open>pair_trsem q r F (t, Running) \<Longrightarrow>
-      hd t = (sc1, ((hl2,hs2),c2)) \<Longrightarrow>
-      F (hlf2, hs2) \<Longrightarrow>
-      hl2 ## hlf2 \<Longrightarrow>
-      ((hl2 + hlf2, hs2), c2) \<midarrow>\<alpha>\<rightarrow> (Inl (hlhlf2', hs2'), c2') \<Longrightarrow>
-      (\<exists>hl2'.
-        hl2' ## hlf2 \<and>
-        hlhlf2' = hl2' + hlf2 \<and>
-        (\<alpha> = Tau \<longrightarrow> hl2' = hl2) \<and>
-        t' = (sc1, ((hl2',hs2'),c2')) # t) \<Longrightarrow>
-      pair_trsem q r F (t', Running)\<close>
-  | crash_leak:
-    \<open>pair_trsem q r F (t, Running) \<Longrightarrow>
-      hd t = (sc1, sc2) \<Longrightarrow>
-      sc1 \<midarrow>|\<rightarrow>               \<and> sc2 \<midarrow>a\<rightarrow> (Inr (), c1') \<or>
-      sc1 \<midarrow>a\<rightarrow> (Inr (), c2') \<and> sc2 \<midarrow>|\<rightarrow>                 \<Longrightarrow>
-      pair_trsem q r F (t, CrashLeak)\<close>
-  | crash_paired:
-    \<open>pair_trsem q r F (t, Running) \<Longrightarrow>
-      hd t = (sc1, sc2) \<Longrightarrow>
-      sc1 \<midarrow>a\<rightarrow> (Inr (), c1') \<Longrightarrow>
-      sc2 \<midarrow>a\<rightarrow> (Inr (), c2') \<Longrightarrow>
-      pair_trsem q r F (t, CrashPair)\<close>
-  | terminate:
-    \<open>pair_trsem q r F (t, Running) \<Longrightarrow>
-      hd t = ((s1, Skip), (s2, Skip)) \<Longrightarrow>
-      q s1 \<Longrightarrow>
-      q s2 \<Longrightarrow>
-      pair_trsem q r F (t, Terminated)\<close>
+    trsem'_init[intro!]:
+    \<open>p s \<Longrightarrow>
+      if c = Skip then rst = Terminated \<and> q s else rst = Running \<Longrightarrow>
+      trsem' p q r g F S c c (AInit (s, rst))\<close>
+  | trsem'_step[intro]:
+    \<open>trsem' p q r g F S cinit c t \<Longrightarrow>
+      ahd t = ((hl, hs), rst) \<Longrightarrow>
+      rst \<noteq> Crashed \<Longrightarrow>
+      rst' = Terminated \<longrightarrow> q s \<Longrightarrow>
+      (case \<gamma> of
+        Loc \<alpha> \<Rightarrow> (\<exists>s'.
+          ((hl, hs), c) \<midarrow>F, \<alpha>\<rightarrow> (s', c') \<and>
+          (case s' of
+            Inr () \<Rightarrow> hl' = hl \<and> hs' = hs \<and> rst' = Crashed
+          | Inl hls' \<Rightarrow>
+              hls' = (hl',hs') \<and>
+              (if c' = Skip then rst' = Terminated else rst' = Running)))
+      | Env \<Rightarrow> hl' = hl \<and> r hs hs' \<and> rst' = rst \<and> rst \<noteq> Crashed) \<Longrightarrow>
+      trsem' p q r g F S cinit c' (ACons ((hl',hs'), rst') \<gamma> t)\<close>
 
-fun safe_trace :: \<open>_ \<Rightarrow> _ \<Rightarrow> _ \<Rightarrow> _ \<Rightarrow> bool\<close> where
-  \<open>safe_trace p g S [] = True\<close>
-| \<open>safe_trace p g S [x] = (p x \<and> S x)\<close>
-| \<open>safe_trace p g S ((hl',hs') # (hl,hs) # t) =
-    (g hs hs' \<and> S (hl',hs') \<and> safe_trace p g S ((hl,hs) # t))\<close>
+inductive_cases trsem_initE[elim!]: \<open>trsem' p q r g F S cinit c (AInit s)\<close>
+inductive_cases trsem_stepE[elim!]: \<open>trsem' p q r g F S cinit c (ACons s' \<alpha> t)\<close>
 
-definition infoleaks :: \<open>_ \<Rightarrow> _ \<Rightarrow> _ \<Rightarrow> _ \<Rightarrow> _ \<Rightarrow> _ \<Rightarrow> _ set\<close> where
-  \<open>infoleaks p q r g S F \<equiv>
-    {t. pair_trsem q r F (t, CrashLeak) \<and> safe_trace p g S t}\<close>
+definition \<open>trsem p q r g F S c \<equiv> {t. \<exists>cx. trsem' p q r g F S c cx t}\<close>
+
+
+\<comment> \<open> TODO: There's a lingering question here over how Env steps are supposed to work. \<close>
+inductive trace_agree
+  :: \<open>('s \<Rightarrow> 'o) \<Rightarrow> ('s, 'a act rgact) alist1 \<Rightarrow> ('s, 'a act rgact) alist1 \<Rightarrow> bool\<close>
+  where
+  tragree_init: \<open>\<bbbA> \<oo> (s1,s2) \<Longrightarrow> trace_agree \<oo> (AInit s1) (AInit s2)\<close>
+| tragree_step_left_tau:
+  \<open>trace_agree \<oo> t1 t2 \<Longrightarrow> trace_agree \<oo> (ACons s1' LocTau t1) t2\<close>
+| tragree_step_right_tau:
+  \<open>trace_agree \<oo> t1 t2 \<Longrightarrow> trace_agree \<oo> t1 (ACons s2' LocTau t2)\<close>
+| tragree_step_env:
+  \<open>trace_agree \<oo> t1 t2 \<Longrightarrow>
+    \<bbbA> \<oo> (s1,s2) \<Longrightarrow>
+    trace_agree \<oo> (ACons s1 Env t1) (ACons s2 Env t2)\<close>
+| tragree_step_vis:
+  \<open>trace_agree \<oo> t1 t2 \<Longrightarrow>
+    \<bbbA> \<oo> (s1,s2) \<Longrightarrow>
+    a1 = a2 \<Longrightarrow>
+    trace_agree \<oo> (ACons s1 (LocVis a1) t1) (ACons s2 (LocVis a2) t2)\<close>
+
+inductive_cases trace_agree_initE[elim!]: \<open>trace_agree \<oo> (AInit s1) (AInit s2)\<close>
+inductive_cases trace_agree_visE[elim!]:
+  \<open>trace_agree \<oo> (ACons s1 (LocVis a1) t1) (ACons s2 (LocVis a2) t2)\<close>
+inductive_cases trace_agree_envE[elim!]:
+  \<open>trace_agree \<oo> (ACons s1 Env t1) (ACons s2 Env t2)\<close>
+
+
+lemma alist1_le_Suc0_iff[simp]:
+  fixes t :: \<open>('a,'b) alist1\<close>
+  shows \<open>size t \<le> Suc 0 \<longleftrightarrow> (\<exists>a. t = AInit a)\<close>
+  by (induct t) (simp add: alist1.size_neq)+
+
+lemma alist1_gt_Suc_iff[simp]:
+  fixes t :: \<open>('a,'b) alist1\<close>
+  shows
+    \<open>0 < k \<Longrightarrow>
+      Suc k \<le> size t \<longleftrightarrow> (\<exists>a b t'. t = ACons a b t' \<and> k \<le> size t')\<close>
+  by (induct t arbitrary: k) simp+
+
 
 lemma security:
   fixes hl1 hl2 :: \<open>'l :: pre_perm_alg\<close>
     and hs1 hs2 :: 's
     and c :: \<open>('l \<times> 's, unit) comm\<close>
+    and p q :: \<open>'l \<times> 's \<Rightarrow> bool\<close>
+    and r g :: \<open>'s \<Rightarrow> 's \<Rightarrow> bool\<close>
   shows
-  \<open>(\<forall>n. safe n (map_comm f c) (Inl ((hl1, hl2), (hs1, hs2))) r g q S F) \<Longrightarrow>
-    infoleaks ((=) (((hl1,hs1),c),((hl2,hs2),c))) q r g S F = {}\<close>
+  \<open>(\<And>n s.
+      (liftP p \<circ> exch4) s \<Longrightarrow>
+      safe n (liftC \<oo> c) (Inl s)
+        (liftR r) (liftR g)
+        (liftP q \<circ> exch4)
+        (liftP S \<circ> exch4) (liftP F \<circ> exch4)) \<Longrightarrow>
+    t1 \<in> trsem p q r g S F c \<Longrightarrow>
+    t2 \<in> trsem p q r g S F c \<Longrightarrow>
+    size t1 \<le> size t2 \<Longrightarrow> \<comment> \<open> wlog \<close>
+    trace_agree (apfst \<oo>) t1 t2\<close>
+  apply (induct t2 arbitrary: t1)
+   apply (clarsimp simp add: trsem_def if_bool_eq_conj)
+   apply (drule_tac x=\<open>1\<close> in meta_spec)
+   apply clarsimp
+
+
   oops
 
 end
